Let 

$$
g(x) := f(x) - \int_{a}^{x} f'(t)\\,dt 
$$

as a function of $x\in [a,b]$, with $a$ fixed. By continuity of $f'$, the function
$g$ is well-defined. By another Fundamental Theorem of Calculus,

$$
g'(x) = f'(x) - \frac{d}{dx}\int_a^x f'(t)\\,dt = f'(x) - f'(x) = 0
$$

at any $x\in [a,b]$, and by the mean value theorem, there then exists
$\xi\in (a, b)$ such that

$$
g(b) - g(a) = g'(\xi)\\, (b-a) = 0
$$

that is, $g(a)=g(b)$ (in fact, $g$ is constant on $[a,b]$). Therefore,

$$
f(a) = g(a) = g(b) = f(b) - \int_{a}^{b} f'(t)\\,dt 
$$

as claimed.
