Let 

$$
g(x) := f(x) - f(a) - \int_{a}^{x} f'(t)\\,dt 
$$

as a function of $x\in I$, with $a$ fixed. By continuity of $f'$, the function
$g$ is well-defined, and that $g(a)=0$. By another Fundamental Theorem of Calculus,

$$
g'(x) = f'(x) - \frac{d}{dx}\int_a^x f'(t)\\,dt = f'(x) - f'(x) = 0
$$

at any $x\in I$, and by the mean value theorem, there then exists
$\xi\in (a, b)$ such that

$$
g(b) - g(a) = g'(\xi)\\, (b-a) = 0
$$

that is, $g(b)=g(a)=0$. It follows that,

$$
g(b) = f(b) - f(a) - \int_{a}^{b} f'(t)\\,dt = 0
$$

as claimed.
