Let 

$$
g(x) := f(x) - \int_{a}^{x} f'(t)\\,dt \\; , \qquad x \in I
$$

with $a$ fixed. By continuity of $f'$, the function $g$ is well-defined, and we are to show $g(b)=g(a)$. Indeed, by another Fundamental Theorem of Calculus, the integral is differentiable with respect to the upper limit, and


$$
\frac{d}{dx}\int_a^x f'(t)\\,dt = f'(x) 
$$

which makes

$$
g'(x) = f'(x) - f'(x) = 0
$$

for all $x\in I$. It follows that $g$ is constant, by an application of the mean value theorem. Indeed, $g(b) - g(a) = g'(\xi) (b - a)$ for some $\xi$ between $a$ and $b$, hence $g(b) = g(a)$. 
